fv/lean/Ragu/Circuits/Element/AllocSquare.lean
@@ -1,5 +1,4 @@
 import Clean.Circuit
-import Clean.Utils.Primes
 import Ragu.Circuits.Core.AllocMul
 
 namespace Ragu.Circuits.Element.AllocSquare
@@ -11,24 +10,27 @@ structure Square (F : Type) where
 deriving ProvableStruct
 
 def main (_input : Unit) : Circuit (F p) (Var Square (F p)) := do
-  let ⟨x, y, z⟩ <- Ragu.Circuits.Core.AllocMul.circuit.main default
+  let ⟨x, y, z⟩ ← subcircuit Ragu.Circuits.Core.AllocMul.circuit default
   assertZero (x - y)
   return ⟨x, z⟩
-
 
 def Assumptions (_input : Unit) := True
 
 def Spec (_input : Unit) (out : Square (F p)) :=
-  out.a_sq = out.a * out.a
+  out.a_sq = out.a^2
 
--- #eval! main (p:=pBabybear) default |>.operations 0
 instance elaborated : ElaboratedCircuit (F p) unit Square where
   main
   localLength _ := 3
 
 theorem soundness : Soundness (F p) elaborated Assumptions Spec := by
   circuit_proof_start
-  sorry
+  simp [Core.AllocMul.circuit, Core.AllocMul.Assumptions, Core.AllocMul.Spec] at h_holds
+  obtain ⟨c1, c2⟩ := h_holds
+  rw [add_neg_eq_zero] at c2
+  rw [←c2] at c1
+  rw [←c1]
+  ring
 
 theorem completeness : Completeness (F p) elaborated Assumptions := by
   sorry
