fv/lean/Ragu/Circuits/Element/Mul.lean
@@ -1,5 +1,4 @@
 import Clean.Circuit
-import Clean.Utils.Primes
 import Ragu.Circuits.Core.AllocMul
 
 namespace Ragu.Circuits.Element.Mul
@@ -11,25 +10,26 @@ structure Input (F : Type) where
 deriving ProvableStruct
 
 def main (input : Var Input (F p)) : Circuit (F p) (Var field (F p)) := do
-  let ⟨x, y, z⟩ <- Ragu.Circuits.Core.AllocMul.circuit.main default
+  let ⟨x, y, z⟩ ← subcircuit Ragu.Circuits.Core.AllocMul.circuit default
   assertZero (x - input.x)
   assertZero (y - input.y)
   return z
-
 
 def Assumptions (_input : Input (F p)) := True
 
 def Spec (input : Input (F p)) (out : field (F p)) :=
   out = input.x * input.y
 
--- #eval! main (p:=pBabybear) default |>.operations 0
 instance elaborated : ElaboratedCircuit (F p) Input field where
   main
   localLength _ := 3
 
 theorem soundness : Soundness (F p) elaborated Assumptions Spec := by
   circuit_proof_start
-  sorry
+  simp [Core.AllocMul.circuit, Core.AllocMul.Assumptions, Core.AllocMul.Spec] at h_holds
+  obtain ⟨c1, c2, c3⟩ := h_holds
+  rw [add_neg_eq_zero] at c2 c3
+  rw [←c2, ←c3, c1]
 
 theorem completeness : Completeness (F p) elaborated Assumptions := by
   sorry
